Add soundness for stable.

Extensions/Semantics/SemanticStable.v
@@ -4,6 +4,11 @@ Require Import Coq.Classes.RelationClasses.
 Require Import Coq.Classes.Equivalence.
 Require Import Coq.Relations.Relation_Definitions.
 Require Import Logic.GeneralLogic.KripkeModel.
+Require Import Logic.ModalLogic.Model.KripkeModel.
+Require Import Logic.SeparationLogic.Model.SeparationAlgebra.
+
+Local Open Scope kripke_model.
+Import KripkeModelNotation_Intuitionistic.
 
 Module SS.
 
@@ -16,24 +21,43 @@ Export SS.
 
 Module Semantics.
 
-Definition stable {worlds: Type} {R: Relation worlds} {EqR: Equivalence R} (X: Ensemble worlds): Prop := forall m n, R m n -> (X m <-> X n).
+Definition stable {worlds: Type} {R: Relation worlds} (X: Ensemble worlds): Prop := forall m n, R m n -> (X m <-> X n).
 
 End Semantics.
 
-Module SemanticsMono.
-
-Definition stable {worlds: Type} {R1: KI.Relation worlds} {R2: Relation worlds} {EqR2: Equivalence R2} (X: MonoEnsemble worlds): Prop := forall m n, R2 m n -> (proj1_sig X m <-> proj1_sig X n).
-
-End SemanticsMono.
-
-Require Import Logic.GeneralLogic.Base.
-
-Local Open Scope kripke_model.
-Import KripkeModelNotation_Intuitionistic.
-
-Class KripkeIntuitionisticStable (L: Language) (MD: Model) {kMD: KripkeModel MD} (M: Kmodel) {R1: KI.Relation (Kworlds M)} {R2: Relation (Kworlds M)} (SM: Semantics L MD): Type := {
-  bis_stable:
+Class KripkeIntuitionisticBisStable (worlds: Type) {R1: KI.Relation worlds} {R2: Relation worlds}: Type := {
+  KI_bis_stable:
     forall m n, R2 m n ->
       (forall m', m <= m' -> exists n', n <= n' /\ R2 m' n') /\
        (forall n', n <= n' -> exists m', m <= m' /\ R2 m' n')
 }.
+
+Class KripkeModalBisStable (worlds: Type) {R1: KM.Relation worlds} {R2: Relation worlds}: Type := {
+  KM_bis_stable:
+    forall m n, R2 m n ->
+      (forall m', KM.Krelation m m' -> exists n', KM.Krelation n n' /\ R2 m' n') /\
+       (forall n', KM.Krelation n n' -> exists m', KM.Krelation m m' /\ R2 m' n')
+}.
+
+Class KripkeModalAbsorbStable (worlds: Type) {R1: KM.Relation worlds} {R2: Relation worlds}: Type := {
+  KM_absorb_stable: forall m n, R1 m n -> R2 m n
+}.
+
+Class SeparationAlgebraBisStable (worlds: Type) {J: Join worlds} {R: Relation worlds}: Type := {
+  split_bis_stable:
+    forall m n, R m n ->
+      (forall m1 m2, join m1 m2 m -> exists n1 n2, join n1 n2 n /\ R m1 n1 /\ R m2 n2) /\
+       (forall n1 n2, join n1 n2 n -> exists m1 m2, join m1 m2 m /\ R m1 n1 /\ R m2 n2);
+  extend_bis_stable:
+    forall m n, R m n ->
+      (forall m1 m2, join m m1 m2 -> exists n1 n2, join n n1 n2 /\ R m1 n1 /\ R m2 n2) /\
+       (forall n1 n2, join n n1 n2 -> exists m1 m2, join m m1 m2 /\ R m1 n1 /\ R m2 n2)
+}.
+
+Require Import Logic.GeneralLogic.Base.
+
+Class SemanticStable (L: Language) (MD: Model) {kMD: KripkeModel MD} (M: Kmodel) {R: Relation (Kworlds M)} (SM: Semantics L MD): Type := {
+  semantic_stable: expr -> Prop;
+  denote_stable: forall x, semantic_stable x <-> Semantics.stable (Kdenotation M x)
+}.
+
