Extensions/Sound/StableSound.v
@@ -1,0 +1,285 @@
+Require Import Coq.Sets.Ensembles.
+Require Import Coq.Logic.Classical_Prop.
+Require Import Coq.Classes.RelationClasses.
+Require Import Coq.Classes.Equivalence.
+Require Import Coq.Relations.Relation_Definitions.
+Require Import Logic.lib.Ensembles_ext.
+Require Import Logic.GeneralLogic.Base.
+Require Import Logic.GeneralLogic.KripkeModel.
+Require Import Logic.ModalLogic.Model.KripkeModel.
+Require Import Logic.SeparationLogic.Model.SeparationAlgebra.
+Require Import Logic.MinimunLogic.Syntax.
+Require Import Logic.PropositionalLogic.Syntax.
+Require Import Logic.ModalLogic.Syntax.
+Require Import Logic.SeparationLogic.Syntax.
+Require Import Logic.Extensions.Semantics.SemanticStable.
+
+Local Open Scope logic_base.
+Local Open Scope syntax.
+Local Open Scope kripke_model.
+Import PropositionalLanguageNotation.
+Import ModalLanguageNotation.
+Import SeparationLogicNotation.
+Import KripkeModelFamilyNotation.
+Import KripkeModelNotation_Intuitionistic.
+
+Module Sound_Trivial.
+
+Require Import Logic.PropositionalLogic.Semantics.Trivial.
+Require Import Logic.ModalLogic.Semantics.Kripke.
+
+Lemma sound_impp_stable {L: Language} {nL: NormalLanguage L} {pL: PropositionalLanguage L} {MD: Model} {kMD: KripkeModel MD} {M: Kmodel} {R: SS.Relation (Kworlds M)} {SM: Semantics L MD} {trSM: TrivialPropositionalSemantics L MD SM} {stableSM: SemanticStable L MD M SM}:
+  forall x y: expr,
+    semantic_stable x -> semantic_stable y -> semantic_stable (x --> y).
+Proof.
+  intros.
+  rewrite denote_stable in H, H0 |- *.
+  unfold Semantics.stable in *.
+  intros.
+  unfold Kdenotation in *; simpl in *.
+  rewrite !(app_same_set (denote_impp _ _)).
+  unfold Semantics.impp; simpl.
+  specialize (H _ _ H1).
+  specialize (H0 _ _ H1).
+  tauto.
+Qed.
+
+Lemma sound_andp_stable {L: Language} {nL: NormalLanguage L} {pL: PropositionalLanguage L} {MD: Model} {kMD: KripkeModel MD} {M: Kmodel} {R: SS.Relation (Kworlds M)} {SM: Semantics L MD} {trSM: TrivialPropositionalSemantics L MD SM} {stableSM: SemanticStable L MD M SM}:
+  forall x y: expr,
+    semantic_stable x -> semantic_stable y -> semantic_stable (x && y).
+Proof.
+  intros.
+  rewrite denote_stable in H, H0 |- *.
+  unfold Semantics.stable in *.
+  intros.
+  unfold Kdenotation in *; simpl in *.
+  rewrite !(app_same_set (denote_andp _ _)).
+  unfold Semantics.andp; simpl.
+  specialize (H _ _ H1).
+  specialize (H0 _ _ H1).
+  tauto.
+Qed.
+
+Lemma sound_orp_stable {L: Language} {nL: NormalLanguage L} {pL: PropositionalLanguage L} {MD: Model} {kMD: KripkeModel MD} {M: Kmodel} {R: SS.Relation (Kworlds M)} {SM: Semantics L MD} {trSM: TrivialPropositionalSemantics L MD SM} {stableSM: SemanticStable L MD M SM}:
+  forall x y: expr,
+    semantic_stable x -> semantic_stable y -> semantic_stable (x || y).
+Proof.
+  intros.
+  rewrite denote_stable in H, H0 |- *.
+  unfold Semantics.stable in *.
+  intros.
+  unfold Kdenotation in *; simpl in *.
+  rewrite !(app_same_set (denote_orp _ _)).
+  unfold Semantics.orp; simpl.
+  specialize (H _ _ H1).
+  specialize (H0 _ _ H1).
+  tauto.
+Qed.
+
+Lemma sound_falsep_stable {L: Language} {nL: NormalLanguage L} {pL: PropositionalLanguage L} {MD: Model} {kMD: KripkeModel MD} {M: Kmodel} {R: SS.Relation (Kworlds M)} {SM: Semantics L MD} {trSM: TrivialPropositionalSemantics L MD SM} {stableSM: SemanticStable L MD M SM}:
+  semantic_stable falsep.
+Proof.
+  intros.
+  rewrite denote_stable.
+  unfold Semantics.stable.
+  intros.
+  unfold Kdenotation.
+  rewrite !(app_same_set denote_falsep).
+  reflexivity.
+Qed.
+
+Lemma sound_boxp_stable {L: Language} {nL: NormalLanguage L} {mL: ModalLanguage L} {MD: Model} {kMD: KripkeModel MD} {M: Kmodel} {R1: KM.Relation (Kworlds M)} {R2: SS.Relation (Kworlds M)} {KMbis: KripkeModalBisStable (Kworlds M)} {SM: Semantics L MD} {kmSM: KripkeModalSemantics L MD M SM} {stableSM: SemanticStable L MD M SM}:
+  forall x: expr,
+    semantic_stable x -> semantic_stable (boxp x).
+Proof.
+  intros.
+  rewrite denote_stable in H |- *.
+  unfold Semantics.stable in *.
+  intros.
+  rewrite !(app_same_set (denote_boxp _)).
+  unfold Semantics.boxp; simpl.
+  pose proof KM_bis_stable _ _ H0.
+  split; intros.
+  + destruct H1 as [_ ?].
+    specialize (H1 _ H3).
+    destruct H1 as [m0 [? ?]].
+    specialize (H2 _ H1).
+    specialize (H _ _ H4).
+    tauto.
+  + rename n0 into m0.
+    destruct H1 as [? _].
+    specialize (H1 _ H3).
+    destruct H1 as [n0 [? ?]].
+    specialize (H2 _ H1).
+    specialize (H _ _ H4).
+    tauto.
+Qed.
+
+Lemma sound_boxp_absorb_stable {L: Language} {nL: NormalLanguage L} {pL: PropositionalLanguage L} {mL: ModalLanguage L} {MD: Model} {kMD: KripkeModel MD} {M: Kmodel} {R1: KM.Relation (Kworlds M)} {R2: SS.Relation (Kworlds M)} {KMabs: KripkeModalAbsorbStable (Kworlds M)} {SM: Semantics L MD} {trSM: TrivialPropositionalSemantics L MD SM} {kmSM: KripkeModalSemantics L MD M SM} {stableSM: SemanticStable L MD M SM}:
+  forall x: expr,
+    semantic_stable x ->
+    (forall (m: Kworlds M), KRIPKE: M, m |= x --> boxp x).
+Proof.
+  intros.
+  rewrite sat_impp, sat_boxp.
+  intros.
+  rewrite denote_stable in H.
+  unfold Semantics.stable in H.
+  apply KM_absorb_stable in H1.
+  specialize (H _ _ H1).
+  tauto.
+Qed.
+
+End Sound_Trivial.
+
+Module Sound_KripkeIntuitionistic.
+
+Require Import Logic.PropositionalLogic.Semantics.Kripke.
+Require Import Logic.ModalLogic.Semantics.Flat.
+Require Import Logic.SeparationLogic.Semantics.FlatSemantics.
+
+Lemma sound_impp_stable {L: Language} {nL: NormalLanguage L} {pL: PropositionalLanguage L} {MD: Model} {kMD: KripkeModel MD} {M: Kmodel} {R1: KI.Relation (Kworlds M)} {R2: SS.Relation (Kworlds M)} {KIbis: KripkeIntuitionisticBisStable (Kworlds M)} {SM: Semantics L MD} {kiSM: KripkeIntuitionisticSemantics L MD M SM} {stableSM: SemanticStable L MD M SM}:
+  forall x y: expr,
+    semantic_stable x -> semantic_stable y -> semantic_stable (x --> y).
+Proof.
+  intros.
+  rewrite denote_stable in H, H0 |- *.
+  unfold Semantics.stable in *.
+  intros.
+  rewrite !(app_same_set (denote_impp _ _)).
+  unfold Semantics.impp; simpl.
+  pose proof KI_bis_stable _ _ H1.
+  split; intros.
+  + destruct H2 as [_ ?].
+    specialize (H2 _ H4).
+    destruct H2 as [m0 [? ?]].
+    specialize (H3 _ H2).
+    specialize (H _ _ H6).
+    specialize (H0 _ _ H6).
+    tauto.
+  + rename n0 into m0.
+    destruct H2 as [? _].
+    specialize (H2 _ H4).
+    destruct H2 as [n0 [? ?]].
+    specialize (H3 _ H2).
+    specialize (H _ _ H6).
+    specialize (H0 _ _ H6).
+    tauto.
+Qed.
+
+Lemma sound_andp_stable {L: Language} {nL: NormalLanguage L} {pL: PropositionalLanguage L} {MD: Model} {kMD: KripkeModel MD} {M: Kmodel} {R1: KI.Relation (Kworlds M)} {R2: SS.Relation (Kworlds M)} {SM: Semantics L MD} {kiSM: KripkeIntuitionisticSemantics L MD M SM} {stableSM: SemanticStable L MD M SM}:
+  forall x y: expr,
+    semantic_stable x -> semantic_stable y -> semantic_stable (x && y).
+Proof.
+  intros.
+  rewrite denote_stable in H, H0 |- *.
+  unfold Semantics.stable in *.
+  intros.
+  rewrite !(app_same_set (denote_andp _ _)).
+  unfold Semantics.andp; simpl.
+  specialize (H _ _ H1).
+  specialize (H0 _ _ H1).
+  tauto.
+Qed.
+
+Lemma sound_orp_stable {L: Language} {nL: NormalLanguage L} {pL: PropositionalLanguage L} {MD: Model} {kMD: KripkeModel MD} {M: Kmodel} {R1: KI.Relation (Kworlds M)} {R2: SS.Relation (Kworlds M)} {SM: Semantics L MD} {kiSM: KripkeIntuitionisticSemantics L MD M SM} {stableSM: SemanticStable L MD M SM}:
+  forall x y: expr,
+    semantic_stable x -> semantic_stable y -> semantic_stable (x || y).
+Proof.
+  intros.
+  rewrite denote_stable in H, H0 |- *.
+  unfold Semantics.stable in *.
+  intros.
+  rewrite !(app_same_set (denote_orp _ _)).
+  unfold Semantics.orp; simpl.
+  specialize (H _ _ H1).
+  specialize (H0 _ _ H1).
+  tauto.
+Qed.
+
+Lemma sound_falsep_stable {L: Language} {nL: NormalLanguage L} {pL: PropositionalLanguage L} {MD: Model} {kMD: KripkeModel MD} {M: Kmodel} {R1: KI.Relation (Kworlds M)} {R2: SS.Relation (Kworlds M)} {SM: Semantics L MD} {kiSM: KripkeIntuitionisticSemantics L MD M SM} {stableSM: SemanticStable L MD M SM}:
+  semantic_stable falsep.
+Proof.
+  intros.
+  rewrite denote_stable.
+  unfold Semantics.stable.
+  intros.
+  rewrite !(app_same_set denote_falsep).
+  reflexivity.
+Qed.
+
+Lemma sound_boxp_stable {L: Language} {nL: NormalLanguage L} {pL: PropositionalLanguage L} {mL: ModalLanguage L} {MD: Model} {kMD: KripkeModel MD} {M: Kmodel} {R1: KI.Relation (Kworlds M)} {R2: KM.Relation (Kworlds M)} {R3: SS.Relation (Kworlds M)} {KMbis: KripkeModalBisStable (Kworlds M)} {SM: Semantics L MD} {fmSM: FlatModalSemantics L MD M SM} {stableSM: SemanticStable L MD M SM}:
+  forall x: expr,
+    semantic_stable x -> semantic_stable (boxp x).
+Proof.
+  intros.
+  rewrite denote_stable in H |- *.
+  unfold Semantics.stable in *.
+  intros.
+  rewrite !(app_same_set (denote_boxp _)).
+  unfold Semantics.boxp; simpl.
+  pose proof KM_bis_stable _ _ H0.
+  split; intros.
+  + destruct H1 as [_ ?].
+    specialize (H1 _ H3).
+    destruct H1 as [m0 [? ?]].
+    specialize (H2 _ H1).
+    specialize (H _ _ H4).
+    tauto.
+  + rename n0 into m0.
+    destruct H1 as [? _].
+    specialize (H1 _ H3).
+    destruct H1 as [n0 [? ?]].
+    specialize (H2 _ H1).
+    specialize (H _ _ H4).
+    tauto.
+Qed.
+
+Lemma sound_boxp_absorb_stable {L: Language} {nL: NormalLanguage L} {pL: PropositionalLanguage L} {mL: ModalLanguage L} {MD: Model} {kMD: KripkeModel MD} {M: Kmodel} {R1: KI.Relation (Kworlds M)} {R2: KM.Relation (Kworlds M)} {R3: SS.Relation (Kworlds M)} {KMabs: KripkeModalAbsorbStable (Kworlds M)} {SM: Semantics L MD} {kiSM: KripkeIntuitionisticSemantics L MD M SM} {fmSM: FlatModalSemantics L MD M SM} {stableSM: SemanticStable L MD M SM}:
+  forall x: expr,
+    semantic_stable x ->
+    (forall (m: Kworlds M), KRIPKE: M, m |= x --> boxp x).
+Proof.
+  intros.
+  rewrite sat_impp.
+  intros.
+  rewrite sat_boxp.
+  intros.
+  rewrite denote_stable in H.
+  unfold Semantics.stable in H.
+  apply KM_absorb_stable in H2.
+  specialize (H _ _ H2).
+  tauto.
+Qed.
+
+Lemma sound_sepcon_stable {L: Language} {nL: NormalLanguage L} {pL: PropositionalLanguage L} {sL: SeparationLanguage L} {MD: Model} {kMD: KripkeModel MD} {M: Kmodel} {R1: KI.Relation (Kworlds M)} {R2: SS.Relation (Kworlds M)} {J: Join (Kworlds M)} {SAbis: SeparationAlgebraBisStable (Kworlds M)} {SM: Semantics L MD} {fsSM: SeparatingSemantics L MD M SM} {stableSM: SemanticStable L MD M SM}:
+  forall x y: expr,
+    semantic_stable x -> semantic_stable y -> semantic_stable (x * y).
+Proof.
+  intros.
+  rewrite denote_stable in H, H0 |- *.
+  unfold Semantics.stable in *.
+  intros.
+  rewrite !(app_same_set (denote_sepcon _ _)).
+  unfold WeakSemantics.sepcon; simpl.
+  pose proof split_bis_stable _ _ H1.
+  split; intros.
+  + destruct H2 as [? _].
+    destruct H3 as [m1 [m2 [? [? ?]]]].
+    specialize (H2 _ _ H3).
+    destruct H2 as [n1 [n2 [? [? ?]]]].
+    exists n1, n2.
+    specialize (H _ _ H6).
+    specialize (H0 _ _ H7).
+    tauto.
+  + destruct H2 as [_ ?].
+    destruct H3 as [n1 [n2 [? [? ?]]]].
+    specialize (H2 _ _ H3).
+    destruct H2 as [m1 [m2 [? [? ?]]]].
+    exists m1, m2.
+    specialize (H _ _ H6).
+    specialize (H0 _ _ H7).
+    tauto.
+Qed.
+
+End Sound_KripkeIntuitionistic.
